coq/Puiseux_base.v
@@ -1,4 +1,4 @@
-(* $Id: Puiseux_base.v,v 1.21 2013-06-16 05:19:30 deraugla Exp $ *)
+(* $Id: Puiseux_base.v,v 1.22 2013-06-16 06:22:35 deraugla Exp $ *)
 
 (* Most of notations are Robert Walker's ones *)
 
@@ -50,11 +50,11 @@ Record term α := { coeff : α; power : Q }.
    computable (therefore proof not constructive). *)
 Axiom series_head : ∀ α, series (term α) → series (term α).
 
-Definition den_divides_comden p comden :=
+Definition den_divides_comden comden p :=
   divide (Pos.to_nat (Qden p)) (comden * Z.abs_nat (Qnum p)).
 
 Definition pow_den_div_com_den α comden (t : term α) :=
-  den_divides_comden (power t) comden.
+  den_divides_comden comden (power t).
 
 Record puiseux_series α :=
   { ps_terms : series (term α);
